Xv6.lean
@@ -1,1 +1,3 @@
 import Xv6.Images
+import Xv6.Image.Facts
+import Xv6.Elf.Kernel
